verified/ARMspartan.dfy
@@ -25,10 +25,10 @@ predicate sp_eq_ops(s1:sp_state, s2:sp_state, o:operand)
 }
 
 function sp_eval_mem(s:state, m:mem):int
-    requires ValidState(s);
-    requires ValidMem(s, m);
+    requires ValidMemState(s.m);
+    requires ValidMem(s.m, m);
     ensures isUInt32(sp_eval_mem(s,m));
-    { MemContents(s, m) }
+    { MemContents(s.m, m) }
 
 function method sp_CNil():codes { CNil }
 function sp_cHead(b:codes):code requires b.sp_CCons? { b.hd }
@@ -78,12 +78,43 @@ function method sp_get_whileBody(c:code):code requires c.While? { c.whileBody }
 //-----------------------------------------------------------------------------
 // Address Helper Functions
 //-----------------------------------------------------------------------------
-function addrval(s:sp_state, a:int):int
+function addrval(s:state, a:int):int
     requires ValidState(s)
-    requires ValidMem(s, Address(a))
+    requires ValidMem(s.m, Address(a))
     ensures isUInt32(addrval(s, a))
 {
-    MemContents(s, Address(a))
+    MemContents(s.m, Address(a))
+}
+
+//-----------------------------------------------------------------------------
+// Useful invariants preserved by instructions
+//-----------------------------------------------------------------------------
+predicate AlwaysInvariant(s:state, s':state)
+{
+    // valid state is maintained
+    ValidState(s) && ValidState(s')
+    // mem validity never changes
+    && (forall m:mem :: m in s.m.addresses <==> m in s'.m.addresses)
+}
+
+predicate ModeInvariant(s:state, s':state)
+{
+    s.mod == s'.mod
+}
+
+predicate AllMemInvariant(s:state, s':state)
+{
+    s.m == s'.m
+}
+
+predicate GlobalsInvariant(s:state, s':state)
+{
+    s.m.globals == s'.m.globals
+}
+
+predicate AddrMemInvariant(s:state, s':state)
+{
+    s.m.addresses == s'.m.addresses
 }
 
 //-----------------------------------------------------------------------------
@@ -141,10 +172,7 @@ function method{:opaque} sp_code_CPS(mod:operand):code
     { Ins(CPS(mod)) }
 
 // Pseudoinstructions  
-function method{:opaque} sp_code_incr(o:operand):code { Ins(ADD(o, o, OConst(1))) }
 function method{:opaque} sp_code_plusEquals(o1:operand, o2:operand):code { Ins(ADD(o1, o1, o2)) }
-function method{:opaque} sp_code_andEquals(o1:operand, o2:operand):code { Ins(AND(o1, o1, o2)) }
-function method{:opaque} sp_code_xorEquals(o1:operand, o2:operand):code { Ins(EOR(o1, o1, o2)) }
 // function method{:opaque} sp_code_push(o:operand):code { 
 //     // Ins(SUB(OSP, OSP, OConst(4)))
 //     var i1 := Ins(SUB(OSP, OSP, OConst(4)));
@@ -168,6 +196,10 @@ lemma sp_lemma_ADD(s:state, r:state, ok:bool,
     requires sp_eval(sp_code_ADD(dst, src1, src2), s, r, ok);
     ensures  evalUpdate(s, dst, OperandContents(s, src1) +
         OperandContents(s, src2), r, ok);
+    ensures ok;
+    ensures AlwaysInvariant(s, r);
+    ensures AllMemInvariant(s, r);
+    ensures ModeInvariant(s, r);
 {
     reveal_sp_eval();
     reveal_sp_code_ADD();
@@ -183,6 +215,10 @@ lemma sp_lemma_SUB(s:state, r:state, ok:bool,
     requires isUInt32(OperandContents(s, src1) - OperandContents(s, src2));
     ensures  evalUpdate(s, dst, OperandContents(s, src1) -
         OperandContents(s, src2), r, ok);
+    ensures ok;
+    ensures AlwaysInvariant(s, r);
+    ensures AllMemInvariant(s, r);
+    ensures ModeInvariant(s, r);
 {
     reveal_sp_eval();
     reveal_sp_code_SUB();
@@ -198,6 +234,10 @@ lemma sp_lemma_MUL(s:state, r:state, ok:bool,
     requires isUInt32(OperandContents(s, src1) * OperandContents(s, src2));
     ensures  evalUpdate(s, dst, OperandContents(s, src1) *
         OperandContents(s, src2), r, ok);
+    ensures ok;
+    ensures AlwaysInvariant(s, r);
+    ensures AllMemInvariant(s, r);
+    ensures ModeInvariant(s, r);
 {
     reveal_sp_eval();
     reveal_sp_code_MUL();
@@ -214,6 +254,10 @@ lemma sp_lemma_UDIV(s:state, r:state, ok:bool,
     requires isUInt32(OperandContents(s, src1) / OperandContents(s, src2));
     ensures  evalUpdate(s, dst, OperandContents(s, src1) /
         OperandContents(s, src2), r, ok);
+    ensures ok;
+    ensures AlwaysInvariant(s, r);
+    ensures AllMemInvariant(s, r);
+    ensures ModeInvariant(s, r);
 {
     reveal_sp_eval();
     reveal_sp_code_UDIV();
@@ -228,6 +272,10 @@ lemma sp_lemma_AND(s:state, r:state, ok:bool,
     requires sp_eval(sp_code_AND(dst, src1, src2), s, r, ok);
     ensures evalUpdate(s, dst, and32(eval_op(s, src1),
         eval_op(s, src2)), r, ok);
+    ensures ok;
+    ensures AlwaysInvariant(s, r);
+    ensures AllMemInvariant(s, r);
+    ensures ModeInvariant(s, r);
 {
     reveal_sp_eval();
     reveal_sp_code_AND();
@@ -242,6 +290,10 @@ lemma sp_lemma_ORR(s:state, r:state, ok:bool,
     requires sp_eval(sp_code_ORR(dst, src1, src2), s, r, ok);
     ensures evalUpdate(s, dst, or32(eval_op(s, src1),
         eval_op(s, src2)), r, ok);
+    ensures ok;
+    ensures AlwaysInvariant(s, r);
+    ensures AllMemInvariant(s, r);
+    ensures ModeInvariant(s, r);
 {
     reveal_sp_eval();
     reveal_sp_code_ORR();
@@ -256,6 +308,10 @@ lemma sp_lemma_EOR(s:state, r:state, ok:bool,
     requires sp_eval(sp_code_EOR(dst, src1, src2), s, r, ok);
     ensures evalUpdate(s, dst, xor32(eval_op(s, src1),
         eval_op(s, src2)), r, ok);
+    ensures ok;
+    ensures AlwaysInvariant(s, r);
+    ensures AllMemInvariant(s, r);
+    ensures ModeInvariant(s, r);
 {
     reveal_sp_eval();
     reveal_sp_code_EOR();
@@ -271,6 +327,10 @@ lemma sp_lemma_ROR(s:state, r:state, ok:bool,
     requires src2.OConst?;
     ensures evalUpdate(s, dst, ror32(eval_op(s, src1),
         eval_op(s, src2)), r, ok);
+    ensures ok;
+    ensures AlwaysInvariant(s, r);
+    ensures AllMemInvariant(s, r);
+    ensures ModeInvariant(s, r);
 {
     reveal_sp_eval();
     reveal_sp_code_ROR();
@@ -286,6 +346,10 @@ lemma sp_lemma_LSL(s:state, r:state, ok:bool,
     requires src2.OConst?;
     ensures evalUpdate(s, dst, shl32(eval_op(s, src1),
         eval_op(s, src2)), r, ok);
+    ensures ok;
+    ensures AlwaysInvariant(s, r);
+    ensures AllMemInvariant(s, r);
+    ensures ModeInvariant(s, r);
 {
     reveal_sp_eval();
     reveal_sp_code_LSL();
@@ -301,6 +365,10 @@ lemma sp_lemma_LSR(s:state, r:state, ok:bool,
     requires src2.OConst?;
     ensures evalUpdate(s, dst, shr32(eval_op(s, src1),
         eval_op(s, src2)), r, ok);
+    ensures ok;
+    ensures AlwaysInvariant(s, r);
+    ensures AllMemInvariant(s, r);
+    ensures ModeInvariant(s, r);
 {
     reveal_sp_eval();
     reveal_sp_code_LSR();
@@ -314,6 +382,10 @@ lemma sp_lemma_MVN(s:state, r:state, ok:bool,
     requires sp_eval(sp_code_MVN(dst, src), s, r, ok);
     ensures evalUpdate(s, dst, not32(eval_op(s, src)),
         r, ok);
+    ensures ok;
+    ensures AlwaysInvariant(s, r);
+    ensures AllMemInvariant(s, r);
+    ensures ModeInvariant(s, r);
 {
     reveal_sp_eval();
     reveal_sp_code_MVN();
@@ -326,6 +398,10 @@ lemma sp_lemma_MOV(s:state, r:state, ok:bool,
     requires ValidDestinationOperand(dst);
     requires sp_eval(sp_code_MOV(dst, src), s, r, ok);
     ensures evalUpdate(s, dst, OperandContents(s, src), r, ok);
+    ensures ok;
+    ensures AlwaysInvariant(s, r);
+    ensures AllMemInvariant(s, r);
+    ensures ModeInvariant(s, r);
 {
     reveal_sp_eval();
     reveal_sp_code_MOV();
@@ -338,9 +414,13 @@ lemma sp_lemma_LDR(s:state, r:state, ok:bool,
     requires ValidOperand(base);
     requires ValidOperand(ofs);
     requires WordAligned(OperandContents(s, base) + OperandContents(s, ofs));
-    requires ValidMem(s, addr_mem(s, base, ofs));
+    requires ValidMem(s.m, addr_mem(s, base, ofs));
     requires sp_eval(sp_code_LDR(rd, base, ofs), s, r, ok);
-    ensures evalUpdate(s, rd, MemContents(s, Address(OperandContents(s, base) + OperandContents(s, ofs))), r, ok)
+    ensures evalUpdate(s, rd, MemContents(s.m, Address(OperandContents(s, base) + OperandContents(s, ofs))), r, ok)
+    ensures ok;
+    ensures AlwaysInvariant(s, r);
+    ensures AllMemInvariant(s, r);
+    ensures ModeInvariant(s, r);
 {
     reveal_sp_eval();
     reveal_sp_code_LDR();
@@ -355,7 +435,11 @@ lemma sp_lemma_LDRglobal(s:state, r:state, ok:bool,
     requires ValidGlobalOffset(g, OperandContents(s, ofs));
     requires AddressOfGlobal(g) == OperandContents(s, base);
     requires sp_eval(sp_code_LDRglobal(rd, g, base, ofs), s, r, ok);
-    ensures evalUpdate(s, rd, GlobalWord(s, g, OperandContents(s, ofs)), r, ok);
+    ensures evalUpdate(s, rd, GlobalWord(s.m, g, OperandContents(s, ofs)), r, ok);
+    ensures ok;
+    ensures AlwaysInvariant(s, r);
+    ensures AllMemInvariant(s, r);
+    ensures ModeInvariant(s, r);
 {
     reveal_sp_eval();
     reveal_sp_code_LDRglobal();
@@ -368,11 +452,14 @@ lemma sp_lemma_STR(s:state, r:state, ok:bool,
     requires ValidOperand(base);
     requires ValidOperand(ofs);
     requires WordAligned(OperandContents(s, base) + OperandContents(s, ofs));
-    requires ValidMem(s, addr_mem(s, base, ofs));
+    requires ValidMem(s.m, addr_mem(s, base, ofs));
     requires sp_eval(sp_code_STR(rd, base, ofs), s, r, ok);
     ensures evalMemUpdate(s, Address(OperandContents(s, base) + OperandContents(s, ofs)),
         OperandContents(s, rd), r, ok)
-    ensures ValidMem(r, addr_mem(s, base, ofs));
+    ensures ok;
+    ensures AlwaysInvariant(s, r);
+    ensures GlobalsInvariant(s, r);
+    ensures ModeInvariant(s, r);
 {
     reveal_sp_eval();
     reveal_sp_code_STR();
@@ -388,6 +475,10 @@ lemma sp_lemma_STRglobal(s:state, r:state, ok:bool,
     requires AddressOfGlobal(g) == OperandContents(s, base);
     requires sp_eval(sp_code_STRglobal(rd, g, base, ofs), s, r, ok);
     ensures evalGlobalUpdate(s, g, OperandContents(s, ofs), OperandContents(s, rd), r, ok);
+    ensures ok;
+    ensures AlwaysInvariant(s, r);
+    ensures ModeInvariant(s, r);
+    ensures AddrMemInvariant(s, r);
 {
     reveal_sp_eval();
     reveal_sp_code_STRglobal();
@@ -399,21 +490,12 @@ lemma sp_lemma_CPS(s:state, r:state, ok:bool, mod:operand)
     requires sp_eval(sp_code_CPS(mod), s, r, ok);
     requires ValidModeEncoding(OperandContents(s, mod));
     ensures  evalModeUpdate(s, OperandContents(s, mod), r, ok);
+    ensures ok;
+    ensures AlwaysInvariant(s, r);
+    ensures AllMemInvariant(s, r);
 {
     reveal_sp_eval();
     reveal_sp_code_CPS();
-}
-
-// Lemmas for frontend functions
-lemma sp_lemma_incr(s:sp_state, r:sp_state, ok:bool, o:operand)
-    requires ValidState(s);
-    requires ValidDestinationOperand(o)
-    requires sp_eval(sp_code_incr(o), s, r, ok)
-    requires isUInt32(eval_op(s, o) + 1);
-    ensures  evalUpdate(s, o, OperandContents(s, o) + 1, r, ok)
-{
-    reveal_sp_eval();
-    reveal_sp_code_incr();
 }
 
 // lemma sp_lemma_push(s:sp_state, r:sp_state, ok:bool, o:operand)
@@ -441,31 +523,13 @@ lemma sp_lemma_plusEquals(s:sp_state, r:sp_state, ok:bool, o1:operand, o2:operan
     requires isUInt32(OperandContents(s, o1) + OperandContents(s, o2));
     ensures evalUpdate(s, o1, OperandContents(s, o1) +
         OperandContents(s, o2), r, ok);
+    ensures ok;
+    ensures AlwaysInvariant(s, r);
+    ensures AllMemInvariant(s, r);
+    ensures ModeInvariant(s, r);
 {
     reveal_sp_eval();
     reveal_sp_code_plusEquals();
-}
-
-lemma sp_lemma_andEquals(s:sp_state, r:sp_state, ok:bool, o1:operand, o2:operand)
-    requires ValidState(s);
-    requires ValidDestinationOperand(o1);
-    requires ValidOperand(o2);
-    requires sp_eval(sp_code_andEquals(o1, o2), s, r, ok);
-    ensures evalUpdate(s, o1, and32(eval_op(s, o1), eval_op(s, o2)), r, ok);
-{
-    reveal_sp_eval();
-    reveal_sp_code_andEquals();
-}
-
-lemma sp_lemma_xorEquals(s:sp_state, r:sp_state, ok:bool, o1:operand, o2:operand)
-    requires ValidState(s);
-    requires ValidDestinationOperand(o1);
-    requires ValidOperand(o2);
-    requires sp_eval(sp_code_xorEquals(o1, o2), s, r, ok);
-    ensures evalUpdate(s, o1, xor32(eval_op(s, o1), eval_op(s, o2)), r, ok);
-{
-    reveal_sp_eval();
-    reveal_sp_code_xorEquals();
 }
 
 lemma sp_lemma_LDRglobaladdr(s:state, r:state, ok:bool, rd:operand, g:operand)
@@ -474,6 +538,10 @@ lemma sp_lemma_LDRglobaladdr(s:state, r:state, ok:bool, rd:operand, g:operand)
     requires ValidGlobal(g);
     requires sp_eval(sp_code_LDRglobaladdr(rd, g), s, r, ok);
     ensures evalUpdate(s, rd, AddressOfGlobal(g), r, ok);
+    ensures ok;
+    ensures AlwaysInvariant(s, r);
+    ensures AllMemInvariant(s, r);
+    ensures ModeInvariant(s, r);
 {
     reveal_sp_eval();
     reveal_sp_code_LDRglobaladdr();
